auto-theories/auto/Lemmas/Wp.v
@@ -15,9 +15,20 @@ From bedrock.auto.Lemmas Require Import
 Local Ltac work :=
   discharge fail idtac fail fail eauto.
 
-Lemma wp_rhs_local (ty : type) : forall ti resolve ρ x Q,
+Section with_resolve.
+  Context {resolve : genv}.
+  Context (ti : thread_info) (ρ : region).
+
+  Notation wp_rhs := (@wp_rhs resolve ti ρ).
+  Notation wp_lhs := (@wp_lhs resolve ti ρ).
+  Notation wp := (@wp resolve ti ρ).
+  Notation wp_decl := (@wp_decl resolve ti ρ).
+  Notation wp_eval_binop := (@wp_eval_binop resolve).
+  Notation wp_eval_unop := (@wp_eval_unop resolve).
+
+Lemma wp_rhs_local (ty : type) : forall x Q,
     Exists v, (tlocal ρ x (tprim (drop_qualifiers ty) v) ** ltrue) //\\ Q v empSP
-    |-- wp_rhs (resolve:=resolve) ti ρ (Ecast Cl2r (Lvalue, Evar (Lname x) ty) ty) Q.
+    |-- wp_rhs (Ecast Cl2r (Lvalue, Evar (Lname x) ty) ty) Q.
 Proof.
   unfold tlocal. intros.
   work.
@@ -40,64 +51,64 @@ Qed.
 
 (* this is the common case for member access
  *)
-Lemma wp_rhs_dot : forall resolve ti x0 obj f fty z Q,
-    wp_lhs (resolve:=resolve) ti x0 obj (fun base free =>
+Lemma wp_rhs_dot : forall obj f fty z Q,
+    wp_lhs obj (fun base free =>
 
        Exists val,
          (_at (_offsetL (_field f) (_eq base)) (tprim (drop_qualifiers fty) val) ** ltrue) //\\
        Q val free)
-    |-- wp_rhs (resolve:=resolve) ti x0 (Ecast Cl2r (Lvalue, Emember obj f fty) z) Q.
+    |-- wp_rhs (Ecast Cl2r (Lvalue, Emember obj f fty) z) Q.
 Proof. Admitted.
 
-Lemma wp_lhs_assign_member_ignore : forall resolve ti r f t obj e t' Q,
-    wp_lhs (resolve:=resolve) ti r obj (fun base free =>
-    wp_rhs (resolve:=resolve) ti r e (fun v' free' =>
+Lemma wp_lhs_assign_member_ignore : forall f t obj e t' Q,
+    wp_lhs obj (fun base free =>
+    wp_rhs e (fun v' free' =>
         _at (_offsetL (_field f) (_eq base)) (uninit (drop_qualifiers t)) **
         (_at (_offsetL (_field f) (_eq base)) (tprim (drop_qualifiers t) v') -*
         Q (free ** free'))))
-    |-- wp_lhs (resolve:=resolve) ti r (Eassign (Emember obj f t) e t') (fun _ free => Q free).
+    |-- wp_lhs (Eassign (Emember obj f t) e t') (fun _ free => Q free).
 Proof. Admitted.
 
 
-Lemma wp_lhs_assign_member : forall resolve ti r f t obj e t' Q,
-    wp_lhs (resolve:=resolve) ti r obj (fun base free =>
-    wp_rhs (resolve:=resolve) ti r e (fun v' free' =>
+Lemma wp_lhs_assign_member : forall f t obj e t' Q,
+    wp_lhs obj (fun base free =>
+    wp_rhs e (fun v' free' =>
         Exists addr, (_offsetL (_field f) (_eq base) &~ addr ** ltrue) //\\
         _at (_eq addr) (tany (drop_qualifiers t)) **
         (_at (_eq addr) (tprim (drop_qualifiers t) v') -* Q addr (free ** free'))))
-    |-- wp_lhs (resolve:=resolve) ti r (Eassign (Emember obj f t) e t') Q.
+    |-- wp_lhs (Eassign (Emember obj f t) e t') Q.
 Proof. Admitted.
 
 
-Theorem wp_call_glob : forall resolve vc ti ρ f ret ts es K PQ F F' ty ty' ty'',
+Theorem wp_call_glob : forall vc f ret ts es K PQ F F' ty ty' ty'',
    (vc = Lvalue \/ vc = Rvalue) ->
    F |-- (|> cglob (resolve:=resolve) f ti (SFunction ret ts PQ)) ** ltrue ->
    F
    |-- wps (wpAnys (resolve:=resolve) ti ρ) es (fun vs free => applyEach ts vs PQ (fun wpp _ =>
             WppD wpp (fun r => K r free))) empSP ** F' ->
    F
-   |-- wp_rhs (resolve:=resolve) ti ρ
+   |-- wp_rhs
          (Ecall (Ecast Cfunction2pointer (vc, Evar (Gname f) ty) ty') es ty'')
          K ** F'.
 Proof. Admitted.
 
 Lemma wp_member_call_glob:
-  forall (resolve : genv) ti ρ (gn : globname) this (ret : type)
+  forall (gn : globname) this (ret : type)
     ty
     (ts : list type) es (K : val -> FreeTemps -> mpred)
     (PQ : val -> arrowFrom val ts WithPrePost) (F F' : mpred)
     cls q,
     F |-- (|> cglob (resolve:=resolve) gn ti (SMethod cls q ret ts PQ)) ** ltrue ->
     F
-    |-- wp_lhs (resolve:=resolve) ti ρ this (fun this =>
+    |-- wp_lhs this (fun this =>
           wps (wpAnys (resolve:=resolve) ti ρ) es (fun (vs : list val) free =>
             applyEach ts vs (PQ this) (fun wpp _ =>
               WppD wpp (fun r => K r free)))) ** F' ->
     F
-    |-- wp_rhs (resolve:=resolve) ti ρ (Emember_call false gn this es ty) K ** F'.
+    |-- wp_rhs (Emember_call false gn this es ty) K ** F'.
 Proof. Admitted.
 
-Theorem wp_constructor_glob : forall resolve ti ρ cname cls ts es K PQ F F' ty,
+Theorem wp_constructor_glob : forall cname cls ts es K PQ F F' ty,
    F |-- (|> cglob (resolve:=resolve) cname ti (SConstructor cls ts PQ)) ** ltrue ->
    F
    |-- wps (wpAnys (resolve:=resolve) ti ρ) es (fun vs free =>
@@ -106,9 +117,7 @@ Theorem wp_constructor_glob : forall resolve ti ρ cname cls ts es K PQ F F' ty,
              Forall a, applyEach ts vs (PQ a) (fun wpp _ =>
                WppD wpp (fun _ => K a free))) empSP ** F' ->
    F
-   |-- wp_rhs (resolve:=resolve) ti ρ
-         (Econstructor cname es ty)
-         K ** F'.
+   |-- wp_rhs (Econstructor cname es ty) K ** F'.
 Proof.
 (*
       intros.
@@ -133,7 +142,7 @@ Proof.
 Admitted.
 
 Theorem wp_decl_class
-: forall resolve ti ρ x ty es cls cname (k : Kpreds -> mpred) ts PQ F F' Q dname PQ',
+: forall x ty es cls cname (k : Kpreds -> mpred) ts PQ F F' Q dname PQ',
     F |-- (|> cglob (resolve:=resolve) cname ti (SConstructor cls ts PQ)) ** ltrue ->
     F |-- (|> cglob (resolve:=resolve) dname ti (SDestructor cls PQ')) ** ltrue ->
     F
@@ -149,12 +158,11 @@ Theorem wp_decl_class
                                 * that is inserted by `SDestructor` *)
                                _local ρ x &~ a ** Q')) Q))))) empSP ** F' ->
     F
-    |-- wp_decl (resolve:=resolve) ti ρ
-                x (Tref cls) (Some (Econstructor cname es ty)) k Q ** F'.
+    |-- wp_decl x (Tref cls) (Some (Econstructor cname es ty)) k Q ** F'.
 Proof. Admitted.
 
 Theorem wp_destroy
-: forall resolve ti this cls F F' Q PQ' dt,
+: forall this cls F F' Q PQ' dt,
     F |-- (|> cglob (resolve:=resolve) (dtor_name dt cls) ti (SDestructor cls PQ')) ** ltrue ->
     F
     |-- (WppD (PQ' this) (fun _ => Q) ** F') ->
@@ -163,35 +171,32 @@ Theorem wp_destroy
 Proof. Admitted.
 
 Lemma wp_rhs_cast_noop:
-  forall (resolve : genv) (ti : thread_info) (ρ : region)
-    (ty : type) (e : Expr) (Q : val -> FreeTemps -> mpred),
-  wp_rhs (resolve:=resolve) ti ρ e Q |-- wp_rhs (resolve:=resolve) ti ρ (Ecast Cnoop (Rvalue, e) ty) Q.
+  forall (ty : type) (e : Expr) (Q : val -> FreeTemps -> mpred),
+  wp_rhs e Q |-- wp_rhs (Ecast Cnoop (Rvalue, e) ty) Q.
 Proof. intros. eapply wpe_cast_noop with (m:=Rvalue). Qed.
 
 Lemma wp_lhs_cast_noop:
-  forall (resolve : genv) (ti : thread_info) (ρ : region)
-    (ty : type) (e : Expr) (Q : val -> FreeTemps -> mpred),
-  wp_lhs (resolve:=resolve) ti ρ e Q |-- wp_lhs (resolve:=resolve) ti ρ (Ecast Cnoop (Lvalue, e) ty) Q.
+  forall (ty : type) (e : Expr) (Q : val -> FreeTemps -> mpred),
+  wp_lhs e Q |-- wp_lhs (Ecast Cnoop (Lvalue, e) ty) Q.
 Proof. intros; eapply wpe_cast_noop with (m:=Lvalue). Qed.
 
-Theorem wp_decl_reference : forall resolve ρ x ty ti init k Q,
-    wp_lhs (resolve:=resolve) ti ρ init (fun a free =>
-             _local ρ x &~ a -* (free ** k (Kfree (_local ρ x &~ a) Q)))
-    |-- wp_decl (resolve:=resolve) ti ρ x (Treference ty) (Some init) k Q.
+Theorem wp_decl_reference : forall x ty init k Q,
+    wp_lhs init (fun a free => _local ρ x &~ a -* (free ** k (Kfree (_local ρ x &~ a) Q)))
+    |-- wp_decl x (Treference ty) (Some init) k Q.
 Proof. reflexivity. Qed.
 
 
-Theorem wp_decl_pointer : forall resolve ρ x ty ti init k Q,
+Theorem wp_decl_pointer : forall x ty init k Q,
     match init with
     | None =>
       Forall a, tlocal_at ρ x a (uninit (Tpointer ty))
               -* k (Kfree (tlocal ρ x (tany (Tpointer ty))) Q)
     | Some init =>
-      wp_rhs (resolve:=resolve) ti ρ init (fun v free =>
+      wp_rhs init (fun v free =>
                  Forall a, tlocal_at ρ x a (tprim (Tpointer ty) v)
               -* (free ** k (Kfree (tlocal ρ x (tany (Tpointer ty))) Q)))
     end
-    |-- wp_decl (resolve:=resolve) ti ρ x (Tpointer ty) init k Q.
+    |-- wp_decl x (Tpointer ty) init k Q.
 Proof.
   simpl; intros. unfold tlocal.
   destruct init.
@@ -210,143 +215,142 @@ Proof.
     reflexivity. }
 Qed.
 
-Theorem wp_decl_int : forall resolve ρ x a b ti init k Q,
+Theorem wp_decl_int : forall x a b init k Q,
     match init with
     | None =>
       tlocal ρ x (uninit (Tint a b)) -* k (Kfree (tlocal ρ x (tany (Tint a b))) Q)
     | Some init =>
-      wp_rhs (resolve:=resolve) ti ρ init (fun v free =>
+      wp_rhs init (fun v free =>
                  tlocal ρ x (tprim (Tint a b) v)
               -* (free ** k (Kfree (tlocal ρ x (tany (Tint a b))) Q)))
     end
-    |-- wp_decl (resolve:=resolve) ti ρ x (Tint a b) init k Q.
+    |-- wp_decl x (Tint a b) init k Q.
 Proof. reflexivity. Qed.
 
-Theorem wp_decl__int : forall resolve ρ x ti init k Q,
+Theorem wp_decl__int : forall x init k Q,
     match init with
     | None =>
       tlocal ρ x (uninit T_int) -* k (Kfree (tlocal ρ x (tany T_int)) Q)
     | Some init =>
-      wp_rhs (resolve:=resolve) ti ρ init (fun v free =>
+      wp_rhs init (fun v free =>
                  tlocal ρ x (tprim T_int v)
               -* (free ** k (Kfree (tlocal ρ x (tany T_int)) Q)))
     end
-    |-- wp_decl (resolve:=resolve) ti ρ x T_int init k Q.
+    |-- wp_decl x T_int init k Q.
 Proof. reflexivity. Qed.
 
-Theorem wp_decl__ulong : forall resolve ρ x ti init k Q,
+Theorem wp_decl__ulong : forall x init k Q,
     match init with
     | None =>
       tlocal ρ x (uninit T_ulong) -* k (Kfree (tlocal ρ x (tany T_ulong)) Q)
     | Some init =>
-      wp_rhs (resolve:=resolve) ti ρ init (fun v free =>
+      wp_rhs init (fun v free =>
                  tlocal ρ x (tprim T_ulong v)
               -* (free ** k (Kfree (tlocal ρ x (tany T_ulong)) Q)))
     end
-    |-- wp_decl (resolve:=resolve) ti ρ x T_ulong init k Q.
+    |-- wp_decl x T_ulong init k Q.
 Proof. reflexivity. Qed.
 
-Theorem wp_decl__int32 : forall resolve ρ x ti init k Q,
+Theorem wp_decl__int32 : forall x init k Q,
     match init with
     | None =>
       tlocal ρ x (uninit T_int32) -* k (Kfree (tlocal ρ x (tany T_int32)) Q)
     | Some init =>
-      wp_rhs (resolve:=resolve) ti ρ init (fun v free =>
+      wp_rhs init (fun v free =>
                  tlocal ρ x (tprim T_int32 v)
               -* (free ** k (Kfree (tlocal ρ x (tany T_int32)) Q)))
     end
-    |-- wp_decl (resolve:=resolve) ti ρ x T_int32 init k Q.
+    |-- wp_decl x T_int32 init k Q.
 Proof. reflexivity. Qed.
 
-Theorem wp_decl_char : forall resolve ρ x a b ti init k Q,
+Theorem wp_decl_char : forall x a b init k Q,
     (let clean := tlocal ρ x (tany (Tchar a b)) in
     match init with
     | None =>
       tlocal ρ x (uninit (Tchar a b)) -* k (Kfree clean Q)
     | Some init =>
-      wp_rhs (resolve:=resolve) ti ρ init (fun v free =>
+      wp_rhs init (fun v free =>
                  tlocal ρ x (tprim (Tchar a b) v)
               -* (free ** k (Kfree clean Q)))
     end)
-    |-- wp_decl (resolve:=resolve) ti ρ x (Tchar a b) init k Q.
+    |-- wp_decl x (Tchar a b) init k Q.
 Proof. reflexivity. Qed.
 
-Theorem wp_decl_bool : forall resolve ρ x ti init k Q,
+Theorem wp_decl_bool : forall x init k Q,
     (let clean := k (Kfree (tlocal ρ x (tany Tbool)) Q) in
     match init with
     | None =>
       tlocal ρ x (uninit Tbool) -* clean
     | Some init =>
-      wp_rhs (resolve:=resolve) ti ρ init (fun v free =>
+      wp_rhs init (fun v free =>
                  tlocal ρ x (tprim Tbool v)
               -* (free ** clean))
     end)
-    |-- wp_decl (resolve:=resolve) ti ρ x Tbool init k Q.
+    |-- wp_decl x Tbool init k Q.
 Proof. reflexivity. Qed.
 
-Theorem wp_decl_qualified : forall resolve ρ x q ty ti init k Q,
-    wp_decl (resolve:=resolve) ti ρ x ty init k Q
-    |-- wp_decl (resolve:=resolve) ti ρ x (Tqualified q ty) init k Q.
+Theorem wp_decl_qualified : forall x q ty init k Q,
+    wp_decl x ty init k Q
+    |-- wp_decl x (Tqualified q ty) init k Q.
 Proof. reflexivity. Qed.
 
-Theorem wp_decl_const : forall resolve ρ x ty ti init k Q,
-    wp_decl (resolve:=resolve) ti ρ x ty init k Q
-    |-- wp_decl (resolve:=resolve) ti ρ x (Qconst ty) init k Q.
+Theorem wp_decl_const : forall x ty init k Q,
+    wp_decl x ty init k Q
+    |-- wp_decl x (Qconst ty) init k Q.
 Proof. reflexivity. Qed.
 
-Theorem wp_decl_mut : forall resolve ρ x ty ti init k Q,
-    wp_decl (resolve:=resolve) ti ρ x ty init k Q
-    |-- wp_decl (resolve:=resolve) ti ρ x (Qmut ty) init k Q.
+Theorem wp_decl_mut : forall x ty init k Q,
+    wp_decl x ty init k Q
+    |-- wp_decl x (Qmut ty) init k Q.
 Proof. reflexivity. Qed.
 
 (* conditions *)
-Lemma wp_lhs_condition : forall resolve ti ρ ty tst th el Q,
-    wp_rhs (resolve:=resolve) ti ρ tst (fun v1 free =>
+Lemma wp_lhs_condition : forall ty tst th el Q,
+    wp_rhs tst (fun v1 free =>
        if is_true v1
-       then wp_lhs (resolve:=resolve) ti ρ th (fun v free' => Q v (free ** free'))
-       else wp_lhs (resolve:=resolve) ti ρ el (fun v free' => Q v (free ** free')))
-    |-- wp_lhs (resolve:=resolve) ti ρ (Eif tst th el ty) Q.
+       then wp_lhs th (fun v free' => Q v (free ** free'))
+       else wp_lhs el (fun v free' => Q v (free ** free')))
+    |-- wp_lhs (Eif tst th el ty) Q.
 Proof. intros; eapply wp_condition with (m:=Lvalue). Qed.
 
-Lemma wp_rhs_condition : forall resolve ti ρ ty tst th el Q,
-    wp_rhs (resolve:=resolve) ti ρ tst (fun v1 free =>
+Lemma wp_rhs_condition : forall ty tst th el Q,
+    wp_rhs tst (fun v1 free =>
       if is_true v1
-      then wp_rhs (resolve:=resolve) ti ρ th (fun v free' => Q v (free ** free'))
-      else wp_rhs (resolve:=resolve) ti ρ el (fun v free' => Q v (free ** free')))
-    |-- wp_rhs (resolve:=resolve) ti ρ (Eif tst th el ty) Q.
+      then wp_rhs th (fun v free' => Q v (free ** free'))
+      else wp_rhs el (fun v free' => Q v (free ** free')))
+    |-- wp_rhs (Eif tst th el ty) Q.
 Proof. intros; eapply wp_condition with (m:=Rvalue). Qed.
 
-Lemma wp_skip : forall (resolve : genv) (ti : thread_info) (ρ : region)
-  (Q : Kpreds),
-    Q.(k_normal) |-- wp (resolve:=resolve) ti ρ Sskip Q.
+Lemma wp_skip : forall (Q : Kpreds),
+    Q.(k_normal) |-- wp Sskip Q.
 Proof. unfold Sskip. intros. rewrite <- wp_seq. reflexivity. Qed.
 
-Lemma wp_return_lhs : forall resolve ti r Q e,
-    wp_lhs (resolve:=resolve) ti r e (finish (fun res : val => k_return Q (Some res)))
-    |-- wp (resolve:=resolve) ti r (Sreturn (Some (Lvalue, e))) Q.
+Lemma wp_return_lhs : forall Q e,
+    wp_lhs e (finish (fun res : val => k_return Q (Some res)))
+    |-- wp (Sreturn (Some (Lvalue, e))) Q.
 Proof. intros. eapply wp_return_val with (c:=Lvalue). Qed.
 
-Lemma wp_return_rhs : forall resolve ti r Q e,
-    wp_rhs (resolve:=resolve) ti r e (finish (fun res : val => k_return Q (Some res)))
-    |-- wp (resolve:=resolve) ti r (Sreturn (Some (Rvalue, e))) Q.
+Lemma wp_return_rhs : forall Q e,
+    wp_rhs e (finish (fun res : val => k_return Q (Some res)))
+    |-- wp (Sreturn (Some (Rvalue, e))) Q.
 Proof. intros. eapply wp_return_val with (c:=Rvalue). Qed.
 
-Theorem wp_lhs_member : forall {resolve} ti r  ty e f Q,
-    wp_lhs (resolve:=resolve) ti r e (fun base free =>
+Theorem wp_lhs_member : forall ty e f Q,
+    wp_lhs e (fun base free =>
         with_addr (_offsetL (_field f) (_eq base)) (fun addr => Q addr free))
-    |-- wp_lhs (resolve:=resolve) ti r (Emember e f ty) Q.
+    |-- wp_lhs (Emember e f ty) Q.
 Proof.
   intros. rewrite <- wp_lhs_member.
   eapply Proper_wp_lhs. red. red. intros.
   rewrite with_addr_defn. reflexivity.
 Qed.
 
-Theorem wp_lhs_subscript : forall {resolve} ti r e i t Q,
-    wp_rhs (resolve:=resolve) ti r e (fun base free =>
-        wp_rhs (resolve:=resolve) ti r i (fun idx free' =>
+Theorem wp_lhs_subscript : forall e i t Q,
+    wp_rhs e (fun base free =>
+        wp_rhs i (fun idx free' =>
           Exists i, [| idx = Vint i |] **
           with_addr (_offsetL (_sub (drop_qualifiers t) i) (_eq base)) (fun addr => Q addr (free' ** free))))
-      |-- wp_lhs (resolve:=resolve) ti r (Esubscript e i t) Q.
+      |-- wp_lhs (Esubscript e i t) Q.
 Proof.
   intros. rewrite <- wp_lhs_subscript.
   eapply Proper_wp_rhs; red; red; intros.
@@ -357,83 +361,105 @@ Proof.
   eapply landL2. reflexivity.
 Qed.
 
-Lemma wp_rhs_unop_wp : forall {resolve} ti r o e ty Q,
-    wp_rhs (resolve:=resolve) ti r e (fun v free =>
-      wp_eval_unop o (drop_qualifiers ty) (drop_qualifiers ty) v (fun v' => Q v' free))
-    |-- wp_rhs (resolve:=resolve) ti r (Eunop o e ty) Q.
+Lemma wp_rhs_unop_wp : forall o e ty Q,
+    wp_rhs e (fun v free =>
+      wp_eval_unop o (drop_qualifiers (type_of e)) (drop_qualifiers ty) v (fun v' => Q v' free))
+    |-- wp_rhs (Eunop o e ty) Q.
 Proof.
   intros.
   setoid_rewrite wp_eval_unop_defn.
-  apply wp_rhs_unop.
+  eapply wp_rhs_unop.
 Qed.
 
-Lemma wp_rhs_binop_wp : forall {resolve} ti r o e1 e2 ty Q,
-    wp_rhs (resolve:=resolve) ti r e1 (fun v1 free1 =>
-      wp_rhs (resolve:=resolve) ti r e2 (fun v2 free2 =>
+Lemma wp_rhs_binop_wp : forall o e1 e2 ty Q,
+    wp_rhs e1 (fun v1 free1 =>
+      wp_rhs e2 (fun v2 free2 =>
         wp_eval_binop o (drop_qualifiers (Typing.type_of e1)) (drop_qualifiers (Typing.type_of e2)) (drop_qualifiers ty) v1 v2 (fun v' => Q v' (free1 ** free2))))
-    |-- wp_rhs (resolve:=resolve) ti r (Ebinop o e1 e2 ty) Q.
+    |-- wp_rhs (Ebinop o e1 e2 ty) Q.
 Proof.
   intros.
   setoid_rewrite wp_eval_binop_defn.
   apply wp_rhs_binop.
 Qed.
 
-Lemma wp_lhs_preinc_wp : forall {resolve} ti r e ty Q,
-    wp_lhs (resolve:=resolve) ti r e (fun a free =>
+Lemma wp_lhs_preinc_wp : forall e ty Q,
+    match companion_type (Typing.type_of e) with
+    | Some cty =>
+    wp_lhs e (fun a free =>
       Exists v',
         _at (_eq a) (tprim (drop_qualifiers ty) v') **
-        wp_eval_binop Badd (drop_qualifiers (Typing.type_of e)) (drop_qualifiers (Typing.type_of e)) (drop_qualifiers ty) v' (Vint 1%Z) (fun v'' =>
+        wp_eval_binop Badd (drop_qualifiers (Typing.type_of e)) cty (drop_qualifiers ty) v' (Vint 1%Z) (fun v'' =>
           _at (_eq a) (tprim (drop_qualifiers ty) v'') -* Q a free))
-    |-- wp_lhs (resolve:=resolve) ti r (Epreinc e ty) Q.
+    | None => lfalse
+    end
+    |-- wp_lhs (Epreinc e ty) Q.
 Proof.
   intros.
   rewrite <-wp_lhs_preinc.
+  destruct (companion_type (type_of e)); auto.
   eapply Proper_wp_lhs; red; red; intros.
   setoid_rewrite wp_eval_binop_defn.
   work.
 Qed.
 
-Lemma wp_lhs_predec_wp : forall {resolve} ti r e ty Q,
-    wp_lhs (resolve:=resolve) ti r e (fun a free =>
+Lemma wp_lhs_predec_wp : forall e ty Q,
+    match companion_type (Typing.type_of e) with
+    | Some cty =>
+    wp_lhs e (fun a free =>
       Exists v',
         _at (_eq a) (tprim (drop_qualifiers ty) v') **
-        wp_eval_binop Bsub (drop_qualifiers (Typing.type_of e)) (drop_qualifiers (Typing.type_of e)) (drop_qualifiers ty) v' (Vint 1%Z) (fun v'' =>
+        wp_eval_binop Bsub (drop_qualifiers (Typing.type_of e)) cty (drop_qualifiers ty) v' (Vint 1%Z) (fun v'' =>
           _at (_eq a) (tprim (drop_qualifiers ty) v'') -* Q a free))
-    |-- wp_lhs (resolve:=resolve) ti r (Epredec e ty) Q.
+    | None => lfalse
+    end
+    |-- wp_lhs (Epredec e ty) Q.
 Proof.
   intros.
   rewrite <-wp_lhs_predec.
+  destruct (companion_type (type_of e)); auto.
   eapply Proper_wp_lhs; red; red; intros.
   setoid_rewrite wp_eval_binop_defn.
   work.
 Qed.
 
-Lemma wp_rhs_postinc_wp : forall {resolve} ti r e ty Q,
-    wp_lhs (resolve:=resolve) ti r e (fun a free =>
+Lemma wp_rhs_postinc_wp : forall e ty Q,
+    match companion_type (type_of e) with
+    | Some cty =>
+    wp_lhs e (fun a free =>
       Exists v',
         _at (_eq a) (tprim (drop_qualifiers ty) v') **
-        wp_eval_binop Badd (drop_qualifiers (Typing.type_of e)) (drop_qualifiers (Typing.type_of e)) (drop_qualifiers ty) v' (Vint 1%Z) (fun v'' =>
+        wp_eval_binop Badd (drop_qualifiers (Typing.type_of e)) cty (drop_qualifiers ty) v' (Vint 1%Z) (fun v'' =>
           _at (_eq a) (tprim (drop_qualifiers ty) v'') -* Q v' free))
-    |-- wp_rhs (resolve:=resolve) ti r (Epostinc e ty) Q.
+    | None => lfalse
+    end
+    |-- wp_rhs (Epostinc e ty) Q.
 Proof.
   intros.
   rewrite <-wp_rhs_postinc.
+  destruct (companion_type (type_of e)); auto.
   eapply Proper_wp_lhs; red; red; intros.
   setoid_rewrite wp_eval_binop_defn.
   work.
 Qed.
 
-Lemma wp_rhs_postdec_wp : forall {resolve} ti r e ty Q,
-    wp_lhs (resolve:=resolve) ti r e (fun a free =>
+Lemma wp_rhs_postdec_wp : forall e ty Q,
+    match companion_type (type_of e) with
+    | Some cty =>
+    wp_lhs e (fun a free =>
       Exists v',
         _at (_eq a) (tprim (drop_qualifiers ty) v') **
-        wp_eval_binop Bsub (drop_qualifiers (Typing.type_of e)) (drop_qualifiers (Typing.type_of e)) (drop_qualifiers ty) v' (Vint 1%Z) (fun v'' =>
+        wp_eval_binop Bsub (drop_qualifiers (Typing.type_of e)) cty (drop_qualifiers ty) v' (Vint 1%Z) (fun v'' =>
           _at (_eq a) (tprim (drop_qualifiers ty) v'') -* Q v' free))
-    |-- wp_rhs (resolve:=resolve) ti r (Epostdec e ty) Q.
+    | None => lfalse
+    end
+    |-- wp_rhs (Epostdec e ty) Q.
 Proof.
   intros.
   rewrite <-wp_rhs_postdec.
+  destruct (companion_type (type_of e)); auto.
   eapply Proper_wp_lhs; red; red; intros.
   setoid_rewrite wp_eval_binop_defn.
   work.
 Qed.
+
+End with_resolve.
